Add a condition indicating that the msf bit is not used in the program & Induction principle with Julay

ImpArrCall.v
@@ -462,6 +462,9 @@ Fixpoint unused (x:string) (c:com) : Prop :=
   | <{{call e}}> => a_unused x e
   end.
 
+Definition unused_prog (x: string) (p:prog) : Prop :=
+  Forall (fun c => unused x c) p.
+
 Open Scope string_scope.
 
 (** As a warm-up we prove that [sel_slh] properly updates the variable "b". *)
@@ -571,6 +574,49 @@ Lemma beval_unused_update : forall X st be n,
   beval (X !-> n; st) be = beval st be.
 Proof. intros X st be n. apply aeval_beval_unused_update. Qed.
 
+Require Import Relations.
+
+(** A non-dependent version of lexicographic ordering. *)
+
+Ltac inv H := inversion H; subst; clear H.
+
+Section LEX_ORDER.
+
+Variable A: Type.
+Variable B: Type.
+Variable ordA: A -> A -> Prop.
+Variable ordB: B -> B -> Prop.
+
+Inductive lex_ord: A*B -> A*B -> Prop :=
+  | lex_ord_left: forall a1 b1 a2 b2,
+      ordA a1 a2 -> lex_ord (a1,b1) (a2,b2)
+  | lex_ord_right: forall a b1 b2,
+      ordB b1 b2 -> lex_ord (a,b1) (a,b2).
+
+Lemma wf_lex_ord:
+  well_founded ordA -> well_founded ordB -> well_founded lex_ord.
+Proof.
+  intros Awf Bwf.
+  assert (forall a, Acc ordA a -> forall b, Acc ordB b -> Acc lex_ord (a, b)).
+  { induction 1. induction 1. constructor; intros. inv H3.
+    - apply H0; auto.
+    - apply H2; auto. }
+  red; intros. destruct a as [a b]. apply H; auto.
+Qed.
+
+Lemma transitive_lex_ord:
+  transitive _ ordA -> transitive _ ordB -> transitive _ lex_ord.
+Proof.
+  intros trA trB; red; intros.
+  inv H; inv H0.
+  - left; eapply trA; eauto.
+  - left; auto.
+  - left; auto.
+  - right; eapply trB; eauto.
+Qed.
+
+End LEX_ORDER.
+
 (** Lexicographic induction *)
 
 Require Import Coq.Arith.Wf_nat.
@@ -659,6 +705,4 @@ Lemma lex_nat_nat_ind (P : nat*nat -> Prop)
 Proof.
   setoid_rewrite <- lex_nat_nat_equiv in IH. now apply lex_ind.
 Qed.
-
-
 
